src/examples/fractional.v
@@ -7,7 +7,6 @@ Undelimit Scope Int_scope.
 
 From iris.base_logic.lib Require Import invariants.
 From lang Require Import lang simp adequacy primitive_laws.
-From examples Require Import rwlock_logic.
 
 From iris.base_logic Require Export base_logic.
 From iris.program_logic Require Export weakestpre.
