src/examples/rwlock.v
@@ -1,6 +1,4 @@
 From iris.base_logic.lib Require Import invariants.
-From lang Require Import lang simp adequacy primitive_laws.
-From examples Require Import rwlock_logic.
 
 From iris.base_logic Require Export base_logic.
 From iris.program_logic Require Export weakestpre.
@@ -11,13 +9,15 @@ From iris.proofmode Require Import reduction.
 From iris.proofmode Require Import ltac_tactics.
 From iris.proofmode Require Import class_instances.
 From iris.program_logic Require Import ectx_lifting.
+
+From lang Require Import lang simp adequacy primitive_laws.
 From lang Require Import notation tactics class_instances.
 From lang Require Import heap_ra.
-From lang Require Import lang.
 From iris Require Import options.
 
 Require Import guarding.guard.
 Require Import guarding.guard_later.
+Require Import guarding.lib.rwlock.
 Require Import examples.misc_tactics.
 
 Definition loop_until e : lang.expr :=
